%        File: curry-howard.tex
%     Created: Mon Feb 10 10:00 AM 2020 E
% Last Change: Mon Feb 10 10:00 AM 2020 E
%
\documentclass[a4paper]{article}
\usepackage{proof}
\usepackage{amsmath}

\title{Towards Curry-Howard Isomorphism}
\author{Chuta Sano}

\begin{document}
\maketitle

\section{Intro}
\paragraph{Scenario}
Imagine if aliens invaded (or peacefully communicated with) Earth. It's quite
intuitive and natural for us to expect our natural languages (eg: English vs
Alienese) to be incompatible and for them not to understand English. This is
because we know that English is an arbitrary language and is something man-made.

\paragraph{}
I suppose we then move to other languages, like math. We believe that math is
universal and thus, although our notations for $\pi$ might not be the same nor
our representation of numbers, we will still be able to know that we ``speak the
same language.'' Again, this falls back to the recurring idea of ``universal''
vs ``arbitrary.''

\paragraph{}
How about programming languages? Is C arbitrary? Answer: yes. Is Java? Yes. Is
Pyth--? Yes. So programming languages are manmade and arbitrary? No.

\paragraph{Claim}
There are universal programming languages that we can discover by following
indisputable universal laws or uncontroversial axioms. In particular, studying
a particular logic gives rise to a programming language. In this paper we will
sketch out the most famous and earliest discovery of such an equivalence -- the
Curry-Howard isomorphism between natural deduction and the simply typed lambda
calculus. The following are equivalent; pick and choose the most appealing
phrase:

\begin{center}
  Propositions are types \\
  Proofs are Programs \\ 
  Logical Systems are Programming Languages \\
\end{center}

\newpage

\paragraph{}
One of the key insights that impacted proof theory from a computational
perspective is the observation that implication, $A \supset B$ (read: $A$
implies $B$), is not just $\neg A \lor B$\footnote{the classical
interpretation}, which treats implication as a mere result of negation and
disjunction.

\paragraph{}
Instead, if we interpret implication as an independent logical connective,
where $A \supset B$ is to be interpreted more naturally: ``if I know $A$, then
I know $B$,'' we obtain a richer presentation of logic, allowing us to observe
the correspondence of logic and computation. In the following presentation, we
will seemingly ``forget'' past results in classical logic that allows us to
present all connectives in terms of $\neg$ and $\land$ (or alternatively, a
``nand'' connective): conjunction, disjunction, and implication are all
independent connectives that cannot be formulated in terms of the other.
However, we will eventually see that we are following an alternate logical
system: \textit{intuitionistic logic}.

\section{Natural Deduction}
\paragraph{}
In proof theory, we study proofs. Whereas in other disciplines, proofs are mere
tools to say something enrichening, in proof theory, we treat proofs as
mathematical objects which allow us to rigorously ``prove'' various properties
of proofs. Natural deduction is one such representation (or a ``model,'' not in
the technical sense) due to Prawitz.

\subsection{Conjunction}
\paragraph{}
We first start with the conjunction (logical and).
$$\infer[(\land I)]{A \land B}{A & B}$$
This is read from top to bottom as a premise to conclusion: the rule says that
from $A$ ``and'' (in a meta sense) $B$, we can conclude $A \land B$. The $(\land
I)$ is a label and is of no theoretical importance; the $I$ is a shorthand for
``introduction''. This is an example of a rule of inference, and more
specifically, an introduction rule since the logical connective $\land$ appears
in the conclusion.

\paragraph{}
Next we have the elimination rules for conjunction. Since an introduction rule
``introduces'' an $\land$ connective to the conclusion, an elimination rule
``eliminates'' an $\land$ connective from the conclusion. At first, we might be
tempted to follow a symmetric pattern:
$$\infer[(\land E_{wrong})]{A \quad B}{A \land B}$$
However, this is not quite what we want -- natural deduction is intentionally
formulated to ``shrink'' down, and so instead, we construct two elimination
rules:

\[
  \infer[(\land E_1)]{A}{A \land B} \quad
  \infer[(\land E_2)]{B}{A \land B}
\]

There might be a concern that we are losing information, but implicitly, since
we know that if we can prove $A \land B$ once, we can prove it again in the
boring fashion (by copy pasting), we can always recover both $A$ and $B$ by
applying $(\land E_1)$ and $(\land E_2)$ respectively to two copies of $A \land
B$, so no information is lost.\footnote{This notion of ``not losing information'' is
called completeness, and indeed there are rigorous ways to verify that the
seemingly arbitrary introduction and elimination rules are correct in that
sense.}

\paragraph{}
So far, we have defined the meaning of a conjunction through the introduction
and elimination rules. As an example of a typical proof in natural deduction, we
will prove the meta theorem that conjunction is associative. That is, we want to
show that from the hypothesis $(A \land B) \land C$, we can conclude $A \land (B
\land C)$ and vice versa. Put concisely, we want to show:
$$(A \land B) \land C \Leftrightarrow A \land (B \land C)$$

$$
\infer[(\land I)]{A \land (B \land C)}{
  \infer[(\land E_1)]{A}{
    \infer[(\land E_1)]{A \land B}{(A \land B) \land C}
  } &
  \infer[(\land I)]{B \land C}{
    \infer[(\land E_2)]{B}{
      \infer[(\land E_1)]{A \land B}{(A \land B) \land C}
  } &
    \infer[(\land E_2)]{C}{(A \land B) \land C)}
  }
}
$$

The opposite direction follows a similar structure (can be an exercise).

\subsection{Implication}
\paragraph{}
Adding implication requires an additional construct in our formulation.
$$\infer[(\supset I)]{A \supset B}{\infer*{B}{[A]}}$$
The premise $\infer*{B}{[A]}$ is called a hypothetical judgement, hypothetical
derivation, or a hypothetical proof. The $[A]$ is a local hypothesis and hence
bound to the hypothetical derivation only -- in particular, this enforces the
intuitive idea that we cannot use $A$ outside of the hypothetical proof.

\paragraph{}
Interestingly, modus ponens appears as a natural elimination rule to the
implication we defined:
$$\infer[(\supset E)]{B}{A \supset B & A}$$

\paragraph{}
At first, we may question the utility of this connective in natural deduction.
Afterall, what's wrong with ignoring $A \supset B$ and instead working directly
with the hypothetical proof? It is indeed true that from a pure ``proof''
perspective, a hypothetical judgement is identical to an implication, and
structurally, using the hypothetical judgement makes more sense, though may not
be economical space-wise. However, do not forget that proof theory is the study
of proofs; this seemingly redundant encoding allows us to look beyond
mere provability since we can now reference proofs at a meta-level (using
hypothetical judgements) and inside the language (using implication).

\subsubsection{Exercise}
Prove the fragment of logic we have introduced so far is ``cartesian closed.''
\footnote{jargon anticipating the connection between logic and category theory}
That is, prove:
$$(A \land B) \supset C \Leftrightarrow A \supset (B \supset C)$$
(implicit parenthesis added for clarity sake)

\subsection{Disjunction}
\paragraph{}
Initially, disjunction seems like a dual to conjunction:
\[
  \infer[(\lor I_1)]{A \lor B}{A} \quad
  \infer[(\lor I_2)]{A \lor B}{B}
\]

However, its elimination rule is a bit complicated:

$$\infer[(\lor E)]{C}{A \lor B & \infer*{C}{[A]} & \infer*{C}{[B]}}$$

This says that to eliminate an instance of an $A \lor B$, we require a motive
$C$ such that from $A$ we can prove $C$ and from $B$ we can prove $C$. This is
essentially a case analysis, which of course is how we intuitively handle
statements like ``$A$ or $B$.''

\subsubsection{Exercise}
Prove that disjunction and conjunction distributes. That is, prove:
$$(A \lor B) \land C \Leftrightarrow (A \land C) \lor (B \land C)$$
and
$$(A \land B) \lor C \Leftrightarrow (A \lor C) \land (B \lor C)$$

\subsection{Sequent}
\paragraph{}
For economic reasons, we will formulate the two dimensional hypothetical
judgements as one dimensional sequents. A sequent $A,B,C,\cdots \vdash D$
consists of a context, a list of antecedents or hypothesis $(A,B,C,\cdots)$, often
abbreviated $\Gamma$, followed by a single conclusion $(D)$.\footnote{An
  intuitionistic interpretation\ldots classical sequents allow a list of
conclusions (interpretted as disjunctions).}

\paragraph{}
For example, recall the introduction rule for implication:
$$\infer[(\supset I)]{A \supset B}{\infer*{B}{[A]}}$$
and rewrite it as follows:
$$\infer[(\supset I)]{\cdot \vdash A \supset B}{A \vdash B}$$
where $\cdot$ is meant to represent an ``empty hypothesis.'' The notion that the
assumption $A$ cannot be used outside the single premise is captured by removing
$A$ from the antecedent in its conclusion.

\paragraph{}
However, this is not quite general enough; in particular, we've ignored the
fact that there can be other hypotheses floating about! That is, since the
conclusion requires an empty hypothesis, we are no longer able to apply this
rule of implication introduction under other hypotheses. Thus, the correct form
of implication introduction should allow arbitrary hypothesis (contexts):
$$\infer[(\supset I)]{\Gamma \vdash A \supset B}{\Gamma, A \vdash B}$$

Again, it's important to note here that $A$ still ``disappears'' in the
conclusion as expected.

\paragraph{}
This one dimensional presentation of hypothetical judgements might further
provoke some dissonance and objections to the role of implication -- really,
what is the difference between $A \vdash B$ and $A \supset B$? From a
syntactical point of view, the difference is clear; $A \vdash B$ is not a
proposition and $A \supset B$ is a proposition. However, this might not be too
satisfying, since afterall, this distinction is something we artificially
created. The reason for this seemingly duplicate work is again because proof
theory is a ``proof-relevant'' theory. We don't only care about something being
true or not or being provable or not -- there is value in looking at an
``implication'' (in an informal sense) from the meta perspective
(sequents/hypothetical judgements) and from the language perspective
$(\supset)$.

\subsubsection{Exercise}
\paragraph{}
Rewrite all (or an arbitrary selection) of the rules of inference keeping in
mind the ``arbitrary context'' rule. For the most part, it's as simple as adding
$\Gamma \vdash$ in front of everything. The only tricky part is the elimination
rule for disjunction, where its hypothetical judgements should be rewritten in a
similar manner to the one in implication introduction.

\paragraph{}
Assuming you did above for at least conjunction introduction (if not, please do
it), try to intuitively convince yourself that what you wrote is general enough
to capture this version of conjunction introduction:
$$\infer{\Gamma_1, \Gamma_2 \vdash A \land B}{\Gamma_1 \vdash A & \Gamma_2
\vdash B}$$ (hint, let your $\Gamma := \Gamma_1, \Gamma_2$ and fill in the
gaps). The filling in of these ``gaps'' is called weakening.



\subsection{Proof Terms}
Are the excercises frustrating enough? So far we have only introduced
metavariables for arbitrary propositions $(A, B, C)$ but have not introduced
metavariables (or any structural way of reasoning) about proof terms.

$$M : A \qquad M \text{ is a proof of proposition } A$$

Similarly, the context now consists of not just propositions but the proof terms
associated with each proposition. Therefore, a typical sequent looks like:

$$x:A, y:B, \cdots \vdash M : A$$
where $\Gamma$ is still used as a metavariable for the hypotheses.

\paragraph{}
This change of course means that we have to reformulate all of our inference
rules.

\subsubsection{Conjunction}
Given a proof of $A$ and a proof of $B$, what constitutes a proof of $A \land
B$? Well, we can form a pair of proofs.

$$\infer[(\land I)]{\Gamma \vdash \langle M,N \rangle : A \land B}{\Gamma \vdash M: A & N : B}$$

On the other hand, if we have an arbitrary proof of $A \land B$, how can we
extract a proof of $A$ and a proof of $B$? Since the proof of $A \land B$ is
arbitrary, we cannot assume its form. Instead, we require two projection
operators $\pi_1$ and $\pi_2$:

\[
  \infer[(\land E_1)]{\Gamma \vdash \pi_1 M : A}{\Gamma \vdash M : A \land B} \quad
  \infer[(\land E_2)]{\Gamma \vdash \pi_2 M : B}{\Gamma \vdash M : A \land B}
\]

\paragraph{$\eta$ expansion}
Note that for any proof term $M : A \land B$, we have
$$M =_{\eta} \langle \pi_1 M, \pi_2 M \rangle$$

The right hand side is called the $\eta$ expansion of $M$. This essentially says
that if we know that $M$ is a proof of $A \land B$, we can create an equivalent
proof by constructing a pair of its first and second projections respectively.
This is also known as ``extensional'' equality, as opposed to structural or
intensional equality, where the idea is that we are asserting that they ought to
be equal because they are observationally equivalent. This is a formal version
of the whole duck principle: if it quacks like a duck, looks like a duck,
\ldots, then it's a duck.

\paragraph{$\beta$ reduction}
On the other hand, for a proof term $\langle M, N \rangle : A \land B$, we can talk about what
happens to the proof term under $\pi_1$ and $\pi_2$.

\begin{gather*}
  \pi_1 \langle M, N \rangle =_{\beta} M \\
  \pi_2 \langle M, N \rangle =_{\beta} N
\end{gather*}

This foreshadows the computational interpretation of natural deduction (of
intuitionistic logic); a $\beta$ reduction of a proof corresponds to a single
``computational step.''

\paragraph{Associativity Proof}
Recall the lengthy and pedantic proof that $(A \land B) \land C \vdash A \land
(B \land C)$. By introducing the syntactical notion of proof terms, we can now
construct a witness that proves the above sequent:

$$x : (A \land B) \land C \vdash \langle \pi_1 \pi_1 x, \langle \pi_2 \pi_1 x,
\pi_2 x \rangle \rangle : A \land (B \land C)$$


\subsubsection{Implication}
\paragraph{}
Implication is the most important logical step that gives us a satisfying
computational interpretation.  Given a hypothetical judgement $M : B$ under
hypothesis $x : A$, we can create a lambda term (or an anonymous function)
$\lambda x:A. M : A \supset B$. It turns out that specifying the type of $x$ is
unnecessary (nevertheless still useful as an annotation), so leaving out the
type annotation, here is the introduction rule:

$$\infer[(\supset I)]{\Gamma \vdash \lambda x.M : A \supset B}{\Gamma, x:A
\vdash M : B}$$

The proof theoretic interpretation is still the same: give me a proof of $A$,
which we will call $x$, and using that, I will prove $B$. However, the
computational interpretation is that of a function: give me some $x : A$ and
I'll give you some well-formed $M : B$.

\paragraph{}
The elimination rule simply puts two proof terms side by side.

$$\infer[(\supset E)]{\Gamma \vdash M\,N : B}{\Gamma \vdash M : A \supset B &
\Gamma \vdash N : A}$$

It may be more suggestive to write $M(N)$ to emphasize that $N$ is applied to
$M$. The computational interpretation is a function application, where $N$ is to
be interpreted as an argument to $M$.

\paragraph{}
For some $M  : A \supset B$, we can conclude
$$M =_{\eta} \lambda x. M x$$

On the other hand for some $M$ and $N$, we have
$$(\lambda x. M) N =_{\beta} [N/x]M$$
where the right hand side is read: ``replace all instances of $x$ in $M$ with
$N$.''

\subsubsection{Disjunction}
\paragraph{}
Whereas conjunction had a notion of projection operators that extracted either
the first or the second term in a pair of proofs, disjunction requires a notion
of injection operators that injects a proof into a disjunction of two proofs:

\[
  \infer[(\lor I_1)]{\Gamma \vdash \iota_1 M : A \lor B}{\Gamma \vdash M : A} \quad
  \infer[(\lor I_2)]{\Gamma \vdash \iota_2 M : A \lor B}{\Gamma \vdash M : B}
\]

\paragraph{}
The elimination rule as we had previously discussed is a case analysis:
$$\infer[(\lor E)]{\Gamma \vdash \text{case}(M; x.P; y.Q) : C}{\Gamma \vdash M : A
\lor B & \Gamma, x : A \vdash P : C & \Gamma, y : B \vdash Q : C}$$

\paragraph{}
The $x.$ and $y.$ at front emphasizes that $P$ and $Q$ depend on $x$ and $y$
respectively.

\paragraph{}
For some $M  : A \supset B$, we can conclude
$$M =_{\eta} \lambda x. M x$$

\end{document}


